wrote theorems for correctness of substitution

theories/AlmostStlc/SemanticsFactsSeq.v
@@ -3,6 +3,8 @@ Require Export SyntaxSeq.
 Require Export SmallStepSeq.
 Require Export DenotationFacts.
 Require Export DenotationSeq.
+Require Export TypesEquiv.
+Require Export MapEFacts.
 Import List.ListNotations.
 Open Scope list_scope.
 From Equations Require Import Equations Signature.
@@ -18,7 +20,7 @@ Inductive covered_in {t2 MR2} (ca : call_syn t2 MR2)
           (E : eval_context t1 MR1 (inr ca) b),  Prop :=
   (* need three base cases, one for each handler style context *)
   | covered_in_mfix_base t MR1 R
-                    (bodies : mfix_bodies nil (R :: MR1) R)
+                    (bodies : mfix_bodies nil MR1 R R)
                     (E : eval_context t (R :: MR1) (inr ca) true) : 
     covered_in ca t _ _ (ev_mfix true R bodies E)
 
@@ -33,7 +35,7 @@ Inductive covered_in {t2 MR2} (ca : call_syn t2 MR2)
     covered_in ca t1 MR1 b E ->
     covered_in ca t2 MR1 b (ev_let E c)
   | covered_in_mfix t MR1 R
-                    (bodies : mfix_bodies nil (R :: MR1) R)
+                    (bodies : mfix_bodies nil MR1 R R)
                     (E : eval_context t (R :: MR1) (inr ca) false) : 
     covered_in ca t (R :: MR1) false E ->
     covered_in ca t _ false (ev_mfix false R bodies E)
@@ -97,13 +99,6 @@ Proof.
   specialize progress_boxed_eval_context with (E := E) as [c' Hc'].
   rewrite Hc'. eexists. reflexivity.
 Qed.
-(*
-Fixpoint equiv_type (t : type) : denote_type t -> denote_type t -> Prop :=
-  match t with 
-  | Nat => eq
-  | Pair t1 t2 => fun '(v1, v2) '(v3, v4) => equiv_type t1 v1 v3 /\ equiv_type t2 v2 v4
-  | Arrow t1 
-*)
 
 Equations var_map_weaken {Γ2} Γ1 (f : forall t, var t Γ1 -> var t Γ2) (hyps : denote_ctx Γ2) : denote_ctx Γ1 :=
   var_map_weaken [] f hyps := tt;
@@ -142,86 +137,132 @@ Proof.
     rewrite <- IHΓ. simp index_ctx. auto.
 Qed.
 
+Lemma ctx_equiv_var_map_weaken:
+  forall (Γ1 Γ2 : ctx) (f : forall t' : vtype, var t' Γ1 -> var t' Γ2) (hyps1 hyps2 : denote_ctx Γ2),
+    ctx_equiv Γ2 hyps1 hyps2 -> ctx_equiv Γ1 (var_map_weaken f hyps1) (var_map_weaken f hyps2).
+Proof.
+  intros Γ1 Γ2 f hyps1 hyps2. generalize dependent Γ2.
+  induction Γ1.
+  - intros. red. auto.
+  - intros Γ2 f hyps1 hyps2 Hhyps. simp var_map_weaken. split; simpl; auto.
+    apply types_equiv_index_ctx. auto.
+Qed.
+
 (* comp_value_mutind *)
 Lemma comp_val_bodies_map : 
   (forall t Γ1 MR (c : comp t Γ1 MR), forall Γ2 (f : forall t', var t' Γ1 -> var t' Γ2) 
-  (hyps : denote_ctx Γ2),
-  denote_comp (comp_map c f) hyps ≈ denote_comp c (var_map_weaken f hyps) ) /\
+  (hyps1 hyps2 : denote_ctx Γ2) (Hhyps : ctx_equiv Γ2 hyps1 hyps2),
+  rutt (mfix_pre_equiv MR) (mfix_post_equiv MR) (types_equiv t) 
+       (denote_comp (comp_map c f) hyps1) (denote_comp c (var_map_weaken f hyps2)) ) /\
   (forall t Γ1 (v : value t Γ1) MR Γ2  (f : forall t', var t' Γ1 -> var t' Γ2) 
-  (hyps : denote_ctx Γ2),
-  denote_value (MR := MR) (val_map v f) hyps ≈ denote_value v (var_map_weaken f hyps)) /\
-  (forall Γ1 MR R (bodies : mfix_bodies Γ1 MR R) Γ2 (f : forall t', var t' Γ1 -> var t' Γ2) 
-      (arg : denote_call_frame R)
-      (hyps : denote_ctx Γ2),
-  denote_bodies (bodies_map bodies f) hyps arg ≈ denote_bodies bodies (var_map_weaken f hyps) arg).
+  (hyps1 hyps2 : denote_ctx Γ2) (Hhyps : ctx_equiv Γ2 hyps1 hyps2),
+      rutt (mfix_pre_equiv MR) (mfix_post_equiv MR) (types_equiv t) 
+           (denote_value (MR := MR) (val_map v f) hyps1) (denote_value v (var_map_weaken f hyps2))) /\
+  (forall Γ1 MR R R' (bodies : mfix_bodies Γ1 MR R R') Γ2 (f : forall t', var t' Γ1 -> var t' Γ2) 
+      (arg1 arg2 : denote_call_frame R') (Harg : call_frame_pre_equiv R' arg1 arg2)
+      (hyps1 hyps2 : denote_ctx Γ2) (Hhyps : ctx_equiv Γ2 hyps1 hyps2),
+      rutt (mfix_pre_equiv (R :: MR)) (mfix_post_equiv (R :: MR)) (call_frame_post_equiv R' arg1 arg2) 
+           (denote_bodies (bodies_map bodies f) hyps1 arg1) (denote_bodies bodies (var_map_weaken f hyps2) arg2)).
 Proof.
   apply comp_value_mutind; intros; auto.
   - rewrite val_map_equation_1. repeat rewrite denote_value_equation_1. 
-    reflexivity.
-  - rewrite val_map_equation_2. repeat rewrite denote_value_equation_2. reflexivity.
-  - rewrite val_map_equation_3. repeat rewrite denote_value_equation_3. rewrite H.
-    setoid_rewrite H0. reflexivity.
+    apply rutt_Ret. reflexivity.
+  - rewrite val_map_equation_2. repeat rewrite denote_value_equation_2. 
+    apply rutt_Ret. constructor.
+  - rewrite val_map_equation_3. repeat rewrite denote_value_equation_3. 
+    eapply rutt_bind; eauto. intros. eapply rutt_bind; eauto. intros.
+    apply rutt_Ret. constructor; auto.
   - rewrite val_map_equation_4. repeat rewrite denote_value_equation_4.
-    rewrite H. setoid_rewrite H0. reflexivity.
+    repeat (eapply rutt_bind; eauto; intros).
+    apply rutt_Ret. constructor; auto.
   - rewrite val_map_equation_5. repeat rewrite denote_value_equation_5.
-    apply eqit_Ret. admit.
+    apply rutt_Ret. simp types_equiv.
+    intros g h Hgh. rewrite <- var_map_weaken_skip. 
+    apply H. constructor; auto.
   - rewrite val_map_equation_6. repeat rewrite denote_value_equation_6.
-    apply eqit_Ret. apply index_weaken.
+    apply rutt_Ret. rewrite <- index_weaken.
+    apply types_equiv_index_ctx. auto.
   - simp comp_map. simp denote_comp.
-  - simp comp_map. simp denote_comp. rewrite H. setoid_rewrite H0.
-    simp var_map_weaken.
-    assert (forall v : denote_type t1, var_map_weaken (var_map_skip f) (v, hyps) = (v, var_map_weaken f hyps)). apply var_map_weaken_skip; auto.
-    eapply eqit_bind. reflexivity. intros. subst. rewrite H1. reflexivity.
+  - simp comp_map. simp denote_comp. 
+    eapply rutt_bind; eauto. intros. rewrite <- var_map_weaken_skip.
+    eapply H0. constructor; auto.
   - simp comp_map. simp denote_comp.
-    rewrite H.
-    eapply eqit_bind. reflexivity. intros. subst.
-    destruct u2; eauto. eapply H0.
-    rewrite H1. rewrite var_map_weaken_skip. reflexivity.
+    eapply rutt_bind; eauto. intros. simp types_equiv in H2. subst r2.
+    destruct r1; auto. rewrite <- var_map_weaken_skip with (t1 := Nat).
+    eapply H1. constructor; auto. reflexivity.
   - simp comp_map. simp denote_comp.
-    rewrite H. eapply eqit_bind. reflexivity.
-    intros. subst. destruct u2. eapply H0.
-    simp var_map_skip. 
-    specialize var_map_weaken_skip with (t1 := List t1) (v := u2) as H2.
-    rewrite <- H2.
-    specialize var_map_weaken_skip with (v := d) (Γ2 := List t1 :: Γ2) 
-      (hyps := (u2, hyps) ) (f := var_map_skip f) as H3.
-    setoid_rewrite <- H3. 
-    simp var_map_weaken. simp index_ctx. simp var_map_skip.
-    simp index_ctx. simp var_map_weaken.
-    admit. (* maybe there are better abstractions and lemmas for reasoning *)
-  - simp comp_map. simp denote_comp. rewrite H.
-    eapply eqit_bind. reflexivity. intros. subst. destruct u2.
-    (* similar to previous *) admit.
-  - simp comp_map. simp denote_comp. rewrite H.
-    eapply eqit_bind. reflexivity. intros. subst.
-    rewrite H0. reflexivity.
-  - simp comp_map. simp denote_comp. rewrite H. reflexivity.
-  - simp comp_map. simp denote_comp. setoid_rewrite H0.
-    (* think carefully about the relation here and might need another
-       properness for interp *)
-    admit.
-Admitted.
+    eapply rutt_bind; eauto. intros. simp types_equiv in H2.
+    dependent destruction H2; eauto.
+    rewrite <- var_map_weaken_skip with (t1 := List t1).
+    setoid_rewrite <- var_map_weaken_skip with (t1 := t1) (Γ2 := List t1 :: Γ2)
+                                       (v := b) 
+                                       (f := var_map_skip f)
+                                       (hyps := (l2, hyps2)).
+    apply H1. repeat split; auto.
+  - simp comp_map. simp denote_comp. 
+    eapply rutt_bind; eauto. intros. simp types_equiv in H1.
+    dependent destruction H1. destruct r1. destruct r2.
+    rewrite <- var_map_weaken_skip with (t1 := t2).
+    setoid_rewrite <- var_map_weaken_skip with (t1 := t1) (Γ2 := t2 :: Γ2)
+                                              (v := d1)
+                                              (f := var_map_skip f)
+                                              (hyps := (d2, hyps2)).
+    apply H0. repeat split; auto.
+  - simp comp_map. simp denote_comp. 
+    do 2 (eapply rutt_bind; eauto; intros).
+  - simp comp_map. simp denote_comp.
+    eapply rutt_bind; eauto. intros. unfold call_term.
+    (* maybe can write a better reasoning principle that encloses this *)
+    destruct (call_mrec x xR r1) as [c1 f1] eqn : Heq1.
+    destruct (call_mrec x xR r2) as [c2 f2] eqn : Heq2. 
+    setoid_rewrite bind_trigger. apply rutt_Vis.
+    eapply mfix_pre_call_mrec; eauto.
+    intros. apply rutt_Ret. eapply mfix_post_equiv_types_equiv; eauto.
+  - simp comp_map. simp denote_comp. 
+    eapply interp_mrec_rutt; eauto.
+  - simp comp_map. simp denote_comp. 
+    apply mapE_rutt. eapply rutt_mon; try eapply H; 
+      intros; try eapply mfix_pre_equiv_lift_handler; try eapply mfix_post_equiv_lift_handler; eauto.
+  - simp comp_map. simp denote_comp.
+    apply mapE_rutt. eapply rutt_mon; try eapply H;
+      intros; try eapply mfix_pre_equiv_perm_handler; try eapply mfix_post_equiv_perm_handler;
+      eauto.
+  - contradiction.
+  - rewrite bodies_map_equation_2.
+    rewrite call_frame_pre_equiv_equation_2 in Harg.
+    dependent destruction Harg; simp denote_bodies.
+    + setoid_rewrite denote_bodies_equation_2.
+      rewrite <- var_map_weaken_skip. 
+      eapply rutt_mon; try eapply H; eauto.
+      intros. constructor; auto. split; auto.
+    + setoid_rewrite denote_bodies_equation_3.
+      eapply rutt_mon; try eapply H0; eauto.
+      intros; constructor; auto.
+Qed.
 
 Lemma comp_map_correct t Γ1 Γ2 MR (c : comp t Γ1 MR) (f : forall t', var t' Γ1 -> var t' Γ2) 
-  (hyps : denote_ctx Γ2) :
-  denote_comp (comp_map c f) hyps ≈ denote_comp c (var_map_weaken f hyps).
+  hyps1 hyps2 : ctx_equiv Γ2 hyps1 hyps2 ->
+                  rutt (mfix_pre_equiv MR) (mfix_post_equiv MR) (types_equiv t) 
+                       (denote_comp (comp_map c f) hyps1) (denote_comp c (var_map_weaken f hyps2)).
 Proof.
   intros. destruct comp_val_bodies_map. auto.
 Qed.
 
 Lemma val_map_correct t Γ1 Γ2 MR (v : value t Γ1) (f : forall t', var t' Γ1 -> var t' Γ2) 
-  (hyps : denote_ctx Γ2) :
-  denote_value (MR := MR) (val_map v f) hyps ≈ denote_value v (var_map_weaken f hyps).
+  (hyps1 hyps2 : denote_ctx Γ2) (Hhyps : ctx_equiv Γ2 hyps1 hyps2) :
+      rutt (mfix_pre_equiv MR) (mfix_post_equiv MR) (types_equiv t) 
+           (denote_value (MR := MR) (val_map v f) hyps1) (denote_value v (var_map_weaken f hyps2)).
 Proof.
-  intros. destruct comp_val_bodies_map as [ ? [? ?] ]. auto.
+  intros. destruct comp_val_bodies_map as [ ? [? ?] ]; auto.
 Qed.
 
-Lemma bodies_map_correct Γ1 Γ2 MR R (bodies : mfix_bodies Γ1 MR R) (f : forall t', var t' Γ1 -> var t' Γ2) 
-      (arg : denote_call_frame R)
-      (hyps : denote_ctx Γ2) : 
-  denote_bodies (bodies_map bodies f) hyps arg ≈ denote_bodies bodies (var_map_weaken f hyps) arg.
+Lemma bodies_map_correct Γ1 Γ2 MR R R' (bodies : mfix_bodies Γ1 MR R R') (f : forall t', var t' Γ1 -> var t' Γ2) 
+      (arg1 arg2 : denote_call_frame R') (Harg : call_frame_pre_equiv R' arg1 arg2)
+      (hyps1 hyps2 : denote_ctx Γ2) (Hhyps : ctx_equiv Γ2 hyps1 hyps2) :
+      rutt (mfix_pre_equiv (R :: MR)) (mfix_post_equiv (R :: MR)) (call_frame_post_equiv R' arg1 arg2) 
+           (denote_bodies (bodies_map bodies f) hyps1 arg1) (denote_bodies bodies (var_map_weaken f hyps2) arg2).
 Proof.
-  intros. destruct comp_val_bodies_map as [ ? [? ?] ]. auto.
+  intros. destruct comp_val_bodies_map as [ ? [? ?] ]; auto.
 Qed.
 
 Equations insert_ctx {t Γ2} Γ1 (v : denote_type t) (hyps : denote_ctx (Γ1 ++ Γ2) ) : 
@@ -241,29 +282,375 @@ Equations hyps_app {Γ2} Γ1 (hyps1 : denote_ctx Γ1) (hyps2 : denote_ctx Γ2) :
   hyps_app _ (v, hyps1) hyps2 := (v, hyps_app _ hyps1 hyps2).
 Arguments hyps_app {_ _}.
 Notation "h1 +++ h2" := (hyps_app h1 h2) (at level 30).
+(* subst_var *)
 
+Definition denote_ctx_single {t} (v : denote_type t) : denote_ctx [t] := (v, tt).
 
-
-
-Lemma subst_correct_aux t u Γ1 Γ2 MR (c : comp u (Γ1 ++ [t] ++ Γ2) MR)  : 
-  forall (v : value t Γ2) (hyps1 : denote_ctx Γ1) (hyps2 : denote_ctx Γ2) v',
-    denote_value (MR := MR) v hyps2 ≈ ret v' ->
-    denote_comp (subst_comp c v) (hyps1 +++ hyps2) ≈
-                denote_comp c (insert_ctx v' (hyps1 +++ hyps2)).
+Theorem denote_value_terminates t Γ MR (v : value t Γ) (hyps : denote_ctx Γ) : 
+  exists vv : denote_type t, denote_value (MR := MR) v hyps ≈ ret vv.
 Proof.
-  (* need dependent induction for compm value and subst,
-     will need reasoning principles for subst_var, and all of the weakings,
-     which means reasoning principle for comp_map
-*)
-  dependent induction c.
-Admitted.
+  induction v.
+  - eexists; setoid_rewrite denote_value_equation_1; eauto. reflexivity.
+  - eexists; setoid_rewrite denote_value_equation_2; eauto. reflexivity.
+  - setoid_rewrite denote_value_equation_3; eauto.
+    specialize (IHv1 hyps) as [vv1 Hvv1].
+    specialize (IHv2 hyps) as [vv2 Hvv2].
+    eexists.
+    rewrite Hvv1. setoid_rewrite bind_ret_l.
+    rewrite Hvv2. setoid_rewrite bind_ret_l. reflexivity.
+  - setoid_rewrite denote_value_equation_4; eauto.
+    specialize (IHv1 hyps) as [vv1 Hvv1].
+    specialize (IHv2 hyps) as [vv2 Hvv2].
+    eexists.
+    rewrite Hvv1. setoid_rewrite bind_ret_l.
+    rewrite Hvv2. setoid_rewrite bind_ret_l. reflexivity.
+  - eexists. setoid_rewrite denote_value_equation_5. reflexivity.
+  - eexists. setoid_rewrite denote_value_equation_6. reflexivity.
+Qed.
+
+Lemma denote_value_ret_equiv:
+  forall (t : vtype) (MR : mfix_ctx) (Γ : ctx) (v : value t Γ) (hyps1 hyps2 : denote_ctx Γ)
+    (vv1 vv2 : denote_type t),
+    ctx_equiv Γ hyps1 hyps2 ->
+    denote_value (MR := MR) v hyps1 ≈ ret vv1 ->
+    denote_value (MR := MR) v hyps2 ≈ ret vv2 ->
+    types_equiv t vv1 vv2.
+Proof.
+  intros t MR Γ2 v.
+  specialize (types_equiv_value_refl _ _ MR v) as Hv.
+  intros hyps1 hyps2 vv1 vv2 Hhyps. specialize (Hv _ _ Hhyps).
+  red in Hv. intros Hvv1 Hvv2. rewrite Hvv1, Hvv2 in Hv.
+  apply rutt_inv_Ret in Hv. auto.
+Qed.
+
+Lemma ctx_equiv_hyps_app Γ1 Γ2 : 
+  forall (hyps11 hyps12 : denote_ctx Γ1) 
+    (hyps21 hyps22 : denote_ctx Γ2),
+    ctx_equiv Γ1 hyps11 hyps12 ->
+    ctx_equiv Γ2 hyps21 hyps22 ->
+    ctx_equiv (Γ1 ++ Γ2) (hyps11 +++ hyps21) (hyps12 +++ hyps22).
+Proof.
+  revert Γ2. induction Γ1.
+  - intros. destruct hyps11. destruct hyps12. simp hyps_app.
+  - intros Γ2 [v1 hyps11] [v2 hyps12] hyps21 hyps22 H1 H2.
+    simp hyps_app. simpl ctx_equiv in H1. destruct H1.
+    constructor; eauto.
+Qed.
+
+Lemma index_ctx_equiv Γ (hyps1 hyps2 : denote_ctx Γ) :
+  (forall t (x : var t Γ), index_ctx x hyps1 = index_ctx x hyps2) -> hyps1 = hyps2.
+Proof.
+  revert hyps1 hyps2. induction Γ; intros.
+  - destruct hyps1. destruct hyps2. auto.
+  - destruct hyps1 as [v1 hyps1]. destruct hyps2 as [v2 hyps2].
+    enough (v1 = v2 /\ hyps1 = hyps2).
+    destruct H0. subst. auto.
+    split.
+    + specialize (H a VarZ). simp index_ctx in H.
+    + apply IHΓ.
+      intros. specialize (H t (VarS x)). simp index_ctx in H.
+Qed.
+
+Equations weaken_denote_ctx Γ1 Γ2 (hyps : denote_ctx (Γ1 ++ Γ2)) : denote_ctx Γ2 :=
+  weaken_denote_ctx nil _ hyps := hyps;
+  weaken_denote_ctx (t :: Γ1) Γ2 (_, hyps) := weaken_denote_ctx Γ1 Γ2 hyps.
+
+Arguments var_map_weaken {_} (_).
+Lemma var_map_weaken_hyps (Γ1 Γ2 : ctx) (hyps : denote_ctx (Γ1 ++ Γ2)) :
+  var_map_weaken Γ2 (weaken_var_l Γ1 Γ2) hyps = weaken_denote_ctx Γ1 Γ2 hyps.
+Proof.
+  generalize dependent Γ2.
+  induction Γ1; simpl.
+  - intros. simp weaken_denote_ctx.
+    induction Γ2; simp var_map_weaken. destruct hyps. auto.
+    destruct hyps as [v hyps]. simp weaken_var_l.
+    simp index_ctx. 
+    erewrite index_ctx_equiv. eauto.
+    intros t x. dependent destruction x.
+    simp index_ctx. auto. simp index_ctx.
+    rewrite <- index_weaken. simp weaken_var_l.
+    simp index_ctx. auto.
+  - intros Γ2 [v hyps]. simp weaken_denote_ctx.
+    rewrite <- IHΓ1. clear IHΓ1.
+    apply index_ctx_equiv. intros t x. 
+    setoid_rewrite <- index_weaken. simp weaken_var_l.
+    simp index_ctx. auto.
+Qed.
+
+Lemma var_map_weaken_single_hyps:
+  forall (t : vtype) (Γ : ctx) (hyps : denote_ctx (t :: Γ)),
+    var_map_weaken _ (weaken_var_l [t] _) hyps = snd hyps.
+Proof.
+  setoid_rewrite var_map_weaken_hyps.
+  intros. destruct hyps as [v hyps]. 
+  simp weaken_denote_ctx. auto.
+Qed.
+
+(* not sure how to correctly write the inductive hyp because it is 
+   dependent, might be easier if subst was  *)
+
+Lemma subst_var_correct t u Γ1 Γ2 MR (v : value t Γ2) (x : var u (Γ1 ++ [t] ++ Γ2 ) ) : 
+  forall (hyps11 hyps12 : denote_ctx Γ1) (hyps21 hyps22 : denote_ctx Γ2) 
+    (Hhyps1 : ctx_equiv _ hyps11 hyps12) (Hhyps2 : ctx_equiv _ hyps21 hyps22) vv,
+    denote_value (MR := MR) v hyps21 ≈ ret vv ->
+    rutt (mfix_pre_equiv MR) (mfix_post_equiv MR) (types_equiv u)
+         (denote_value (val_var x) (hyps11 +++ ((denote_ctx_single vv) +++ hyps21) ) )
+         (denote_value (subst_var Γ1 Γ2 v x) (hyps12 +++ hyps22) ).
+Proof.
+  revert x v. generalize dependent Γ2. 
+  induction Γ1.
+  - simpl app. intros Γ2 x v [] [] hyps21 hyps22 _ Hhyps2 vv Hvv. simp hyps_app.
+    dependent destruction x.
+    + simp subst_var. setoid_rewrite denote_value_equation_6. 
+      setoid_rewrite hyps_app_equation_2.
+      setoid_rewrite index_ctx_equation_1.
+      destruct (denote_value_terminates _ _ MR v hyps22) as [vv' Hvv'].
+      rewrite Hvv'. apply rutt_Ret. eapply denote_value_ret_equiv; eauto.
+    + setoid_rewrite hyps_app_equation_2. setoid_rewrite denote_value_equation_6.
+      simp hyps_app. 
+      setoid_rewrite index_ctx_equation_2. destruct Γ2.
+      * inversion x.
+      * simp subst_var. setoid_rewrite denote_value_equation_6.
+        apply rutt_Ret. apply types_equiv_index_ctx. auto.
+  - simpl app. intros Γ2 x v hyps11 hyps12 hyps21 hyps22 Hhyps1 Hhyps2 vv Hvv.
+    dependent destruction x.
+    + simp subst_var. setoid_rewrite denote_value_equation_6. clear IHΓ1.
+      apply rutt_Ret. destruct hyps11. destruct hyps12. red in Hhyps1. dependent destruction Hhyps1.
+      simp hyps_app.
+    + simp subst_var. red in Hhyps1. dependent destruction Hhyps1.
+      eapply IHΓ1 with (x := x) in Hvv; eauto. 
+      setoid_rewrite denote_value_equation_6. 
+      setoid_rewrite denote_value_equation_6 in Hvv. 
+      destruct hyps11 as [t0 hyps11]. simp hyps_app. simp index_ctx.
+      simpl snd in Hvv. rewrite Hvv.
+      clear Hvv. unfold weaken_l_value_single,weaken_l_value.
+      assert (Hhyps' : ctx_equiv ((a :: Γ1) ++ Γ2) (hyps12 +++ hyps22) (hyps12 +++ hyps22)).
+      {
+        apply ctx_equiv_hyps_app; auto. 
+        transitivity ((t0,hyps11)); eauto. constructor; auto.
+        symmetry. auto. symmetry. auto.
+        constructor; auto.
+        transitivity hyps21; auto. symmetry. auto.
+      }
+      rewrite val_map_correct with (hyps2 := hyps12 +++ hyps22); auto.
+      enough (var_map_weaken _ (weaken_var_l [a] (Γ1 ++ Γ2)) (hyps12 +++ hyps22) =
+                snd hyps12 +++ hyps22).
+      setoid_rewrite H.
+      apply types_equiv_value_refl; auto. 
+      destruct hyps12 as [v1 hyps12].
+      simpl. apply ctx_equiv_hyps_app; auto.
+      etransitivity; eauto. symmetry. auto.
+      etransitivity; eauto. symmetry. auto.
+      rewrite var_map_weaken_single_hyps.
+      destruct hyps12. simp hyps_app.
+      auto.
+Qed.
+
+(* further generalize hyps stuff *)
+Lemma subst_correct_aux_prod :
+  (forall u Γ MR (c : comp u Γ MR) Γ1 t Γ2 (v : value t Γ2) 
+     (hyps11 hyps12 : denote_ctx Γ1) (hyps21 hyps22 : denote_ctx Γ2) vv (c' : comp u (Γ1 ++ [t] ++ Γ2) MR) ,
+      ctx_equiv Γ1 hyps11 hyps12 ->
+      ctx_equiv Γ2 hyps21 hyps22 ->
+      Γ = Γ1 ++ [t] ++ Γ2 ->
+      c ~= c' ->
+      (forall MR, denote_value (MR := MR) v hyps21 ≈ ret vv) ->
+      comp_equiv_rutt (denote_comp (subst_comp c' v) (hyps11 +++ hyps21))
+                      (denote_comp c' (hyps12 +++ ((denote_ctx_single vv) +++ hyps22)) )) /\
+  (forall u Γ (v0 : value u Γ) MR Γ1 t Γ2 (v : value t Γ2)
+     (hyps11 hyps12 : denote_ctx Γ1) (hyps21 hyps22 : denote_ctx Γ2) vv 
+     (v0' : value u (Γ1 ++ [t] ++ Γ2)),
+      ctx_equiv Γ1 hyps11 hyps12 ->
+      ctx_equiv Γ2 hyps21 hyps22 ->
+      Γ = Γ1 ++ [t] ++ Γ2 ->
+      v0 ~= v0' ->
+      (forall MR, denote_value (MR := MR) v hyps21 ≈ ret vv) ->
+      comp_equiv_rutt (MR := MR) (denote_value (subst_value v0' v) (hyps11 +++ hyps21) )
+                      (denote_value v0' (hyps12 +++ ((denote_ctx_single vv) +++ hyps22))) ) /\
+  (forall Γ MR R R' (bodies : mfix_bodies Γ MR R R') Γ1 t Γ2 (v : value t Γ2)
+     (hyps11 hyps12 : denote_ctx Γ1) (hyps21 hyps22 : denote_ctx Γ2) vv 
+     (bodies' : mfix_bodies (Γ1 ++ [t] ++ Γ2) MR R R')
+     (arg1 arg2 : denote_call_frame R') (Harg : call_frame_pre_equiv R' arg1 arg2),
+      ctx_equiv Γ1 hyps11 hyps12 ->
+      ctx_equiv Γ2 hyps21 hyps22 ->
+      Γ = Γ1 ++ [t] ++ Γ2 ->
+      bodies ~= bodies' ->
+      (forall MR, denote_value (MR := MR) v hyps21 ≈ ret vv) ->
+      rutt (mfix_pre_equiv (R :: MR)) (mfix_post_equiv (R :: MR)) 
+           (call_frame_post_equiv R' arg1 arg2)  
+           (denote_bodies (subst_bodies bodies' v) (hyps11 +++ hyps21) arg1 )
+           (denote_bodies bodies' (hyps12 +++ ((denote_ctx_single vv) +++ hyps22)) arg2 )
+)
+.
+Proof.
+  eapply comp_value_mutind; intros; subst.
+  - setoid_rewrite subst_value_equation_1.
+    setoid_rewrite denote_value_equation_1. apply rutt_Ret.
+    reflexivity.
+  - setoid_rewrite subst_value_equation_2.
+    setoid_rewrite denote_value_equation_2. apply rutt_Ret.
+    constructor.
+  - setoid_rewrite subst_value_equation_3.
+    setoid_rewrite denote_value_equation_3. red.
+    eapply rutt_bind; eauto. eapply H; eauto.
+    intros. eapply rutt_bind; eauto. eapply H0; eauto.
+    intros. apply rutt_Ret.
+    constructor; auto.
+  - setoid_rewrite subst_value_equation_4.
+    setoid_rewrite denote_value_equation_4.
+    eapply rutt_bind. eapply H; eauto.
+    intros. eapply rutt_bind. eapply H0; eauto.
+    intros. apply rutt_Ret. constructor; auto.
+  - setoid_rewrite subst_value_equation_5.
+    setoid_rewrite denote_value_equation_5.
+    apply rutt_Ret. simp types_equiv.
+    intros x y Hxy.
+    specialize (H (t1 :: Γ1) t Γ2 v (x, hyps11) (y, hyps12) hyps21 hyps22 vv). 
+    assert (ctx_equiv (t1 :: Γ1) (x, hyps11) (y, hyps12)).
+    constructor; auto.
+    specialize (H cbody H2 H1 eq_refl JMeq_refl H4).
+    simp hyps_app in H. rewrite H.
+    apply types_equiv_comp_refl. cbn.
+    constructor. etransitivity; eauto. symmetry. auto.
+    simpl. apply ctx_equiv_hyps_app.
+    etransitivity; eauto. symmetry. auto.
+    unfold denote_ctx_single. simp hyps_app.
+    cbn. constructor; auto.
+    2 : etransitivity; eauto; symmetry; auto.
+    simpl. 
+    eapply denote_value_ret_equiv with 
+      (v := v) (hyps1 := hyps21) (hyps2 := hyps21); eauto.
+    etransitivity; eauto; symmetry; auto.
+  - setoid_rewrite subst_value_equation_6.
+    specialize (H3 MR).
+    eapply subst_var_correct with (x := x)in H3 as H4; eauto.
+    assert (Hsubst : comp_equiv_rutt (MR := MR)
+              (denote_value (subst_var Γ1 Γ2 v x) (hyps11 +++ hyps21))
+              (denote_value (subst_var Γ1 Γ2 v x) (hyps12 +++ hyps22))).
+    { apply types_equiv_value_refl. apply ctx_equiv_hyps_app; auto. }
+    rewrite Hsubst. rewrite <- H4.
+    apply types_equiv_value_refl.
+    apply ctx_equiv_hyps_app; auto.
+    apply ctx_equiv_hyps_app; auto. constructor; auto.
+    2 : constructor. simpl.
+    eapply denote_value_ret_equiv with (hyps1 := hyps21) (hyps2 := hyps21); eauto.
+    etransitivity; eauto. symmetry; auto.
+  - setoid_rewrite subst_comp_equation_1. 
+    setoid_rewrite denote_comp_equation_1. eauto.
+  - setoid_rewrite subst_comp_equation_2.
+    setoid_rewrite denote_comp_equation_2.
+    eapply rutt_bind; eauto. eapply H; eauto.
+    intros. setoid_rewrite <- hyps_app_equation_2.
+    specialize (H0 (t1 :: Γ1)). eapply H0; eauto.
+    constructor; auto.
+  - setoid_rewrite subst_comp_equation_3. 
+    setoid_rewrite denote_comp_equation_3.
+    eapply rutt_bind. eapply H; eauto.
+    intros. simp types_equiv in H4. subst r2. destruct r1.
+    eapply H0; eauto.
+    specialize (H1 (Nat :: Γ1) t0 Γ2 v (r1, hyps11) (r1, hyps12) ). 
+    setoid_rewrite hyps_app_equation_2 in H1. eapply H1; eauto.
+    constructor; auto. reflexivity.
+ - setoid_rewrite subst_comp_equation_4.
+   setoid_rewrite denote_comp_equation_4.
+   eapply rutt_bind. eapply H; eauto. intros.
+   simp types_equiv in H4. dependent destruction H4.
+   eapply H0; eauto. clear H. clear H0.
+   specialize (H1 (t1 :: List t1 :: Γ1) t Γ2 v (a, (l1, hyps11)) (b, (l2, hyps12))).
+   repeat setoid_rewrite hyps_app_equation_2 in H1.
+   setoid_rewrite hyps_app_equation_1 in H1. setoid_rewrite hyps_app_equation_2.
+   setoid_rewrite hyps_app_equation_1.
+   eapply H1; eauto. repeat constructor; auto.
+ - setoid_rewrite subst_comp_equation_5.
+   setoid_rewrite denote_comp_equation_5.
+   eapply rutt_bind. eapply H; eauto. intros.
+   destruct r1 as [v1 v2]. destruct r2 as [v3 v4].
+   simp types_equiv in H3. dependent destruction H3.
+   cbn in fst_rel. cbn in snd_rel.
+   clear H.
+   specialize (H0 (t1 :: t2 :: Γ1) t Γ2 v (v1, (v2, hyps11)) (v3, (v4, hyps12)) ).
+   repeat setoid_rewrite hyps_app_equation_2 in H0. 
+   setoid_rewrite hyps_app_equation_1 in H0.
+   setoid_rewrite hyps_app_equation_2. setoid_rewrite hyps_app_equation_1. 
+   eapply H0; auto. repeat constructor; auto.
+ - setoid_rewrite subst_comp_equation_6.
+   setoid_rewrite denote_comp_equation_6.
+   eapply rutt_bind; eauto. eapply H; eauto.
+   intros. eapply rutt_bind. eapply H0; eauto. intros. 
+   simp types_equiv in H3.
+ - setoid_rewrite subst_comp_equation_7.
+   setoid_rewrite denote_comp_equation_7.
+   eapply rutt_bind. eapply H; eauto.
+   intros. unfold call_term.
+   destruct (call_mrec x xR r1) as [c1 f1] eqn : Heq1.
+   destruct (call_mrec x xR r2) as [c2 f2] eqn : Heq2. 
+   setoid_rewrite bind_trigger. apply rutt_Vis.
+   eapply mfix_pre_call_mrec; eauto.
+   intros. apply rutt_Ret. eapply mfix_post_equiv_types_equiv; eauto.
+ - setoid_rewrite subst_comp_equation_8.
+   setoid_rewrite denote_comp_equation_8.
+   eapply interp_mrec_rutt
+     with (RPreInv := call_frame_pre_equiv R)
+          (RPostInv := call_frame_post_equiv R);
+     intros; try eapply H0; eauto.
+ - setoid_rewrite subst_comp_equation_9.
+   setoid_rewrite denote_comp_equation_9.
+   apply mapE_rutt.
+   eapply rutt_mon; try eapply H; eauto.
+   intros; eapply mfix_pre_equiv_lift_handler; eauto.
+   intros; eapply mfix_post_equiv_lift_handler; eauto.
+ - setoid_rewrite subst_comp_equation_10.
+   setoid_rewrite denote_comp_equation_10.
+   apply mapE_rutt.
+   eapply rutt_mon; try eapply H; eauto.
+   intros; eapply mfix_pre_equiv_perm_handler; eauto.
+   intros; eapply mfix_post_equiv_perm_handler; eauto.
+ - inversion arg1.
+ - rewrite call_frame_pre_equiv_equation_2 in Harg.
+   rewrite subst_bodies_equation_2.
+   dependent destruction Harg.
+   + setoid_rewrite denote_bodies_equation_2.
+     setoid_rewrite <- hyps_app_equation_2.
+     specialize (H (t1 :: Γ1) t Γ2 v (a1, hyps11) (a2, hyps12)).
+     specialize (H hyps21 hyps22 vv body).
+     assert (Hahyps : ctx_equiv (t1 :: Γ1) (a1, hyps11) (a2, hyps12)).
+     constructor; auto.
+     specialize (H Hahyps H3 eq_refl JMeq_refl H5).
+     eapply rutt_mon; try eapply H; eauto.
+     intros. constructor; auto.
+   + setoid_rewrite denote_bodies_equation_3.
+     eapply rutt_mon; try eapply H0; eauto.
+     intros. constructor; auto.
+     Unshelve. eauto.
+Qed.
+
+Theorem subst_comp_correct t u Γ1 Γ2 MR (c : comp u (Γ1 ++ [t] ++ Γ2) MR) (v : value t Γ2)
+        (hyps11 hyps12 : denote_ctx Γ1) (hyps21 hyps22 : denote_ctx Γ2) vv :
+  ctx_equiv Γ1 hyps11 hyps12 ->
+  ctx_equiv Γ2 hyps21 hyps22 ->
+  (forall MR, denote_value (MR := MR) v hyps21 ≈ ret vv) ->
+  comp_equiv_rutt (denote_comp (subst_comp c v) (hyps11 +++ hyps21))
+                  (denote_comp c (hyps12 +++ ((denote_ctx_single vv) +++ hyps22)) ).
+Proof.
+  destruct subst_correct_aux_prod as [H _].
+  intros. eapply H; eauto.
+Qed.
 
 Theorem subst_correct t u Γ MR (c : comp u (t :: Γ) MR) (v : value t Γ) : 
-  forall (hyps : denote_ctx Γ) v',
-    denote_value (MR := MR) v hyps ≈ ret v' ->
-    denote_comp (subst_comp_cons c v) hyps ≈
-                denote_comp c (v', hyps).
+  forall (hyps1 hyps2 : denote_ctx Γ) vv,
+    ctx_equiv Γ hyps1 hyps2->
+    (forall MR, denote_value (MR := MR) v hyps1 ≈ ret vv) ->
+    comp_equiv_rutt 
+      (denote_comp (subst_comp_cons c v) hyps1)
+                (denote_comp c (vv, hyps2)).
 Proof.
-  intros. specialize (subst_correct_aux t u nil Γ MR c v tt _ _ H) as Heq.
-  simp hyps_app in Heq.
+  intros. 
+  specialize subst_comp_correct with 
+    (Γ1 := []) (Γ2 := Γ) 
+    (hyps11 := tt) (hyps12 := tt)
+    as Hsubst. 
+  setoid_rewrite hyps_app_equation_1 in Hsubst.
+  setoid_rewrite hyps_app_equation_2 in Hsubst.
+  setoid_rewrite hyps_app_equation_1 in Hsubst. 
+  eapply Hsubst; eauto. constructor.
 Qed.
