theories/AlmostStlc/TypesEquiv.v
@@ -8,6 +8,7 @@ Require Export Rutt.
 Require Export RuttFacts.
 Require Import ITree.Basics.HeterogeneousRelations.
 Require Export InterpMTreeFacts.
+Require Export MapEFacts.
 Import List.ListNotations.
 Open Scope list_scope.
 From Equations Require Import Equations Signature.
@@ -25,7 +26,7 @@ From Coq Require Import
 
 Inductive list_rel {A} (R : Rel A A): Rel (list A) (list A) :=
   | list_rel_nil : list_rel R nil nil
-  | list_rel_cons a b l1 l2 : R a b ->list_rel R l1 l2 -> list_rel R (cons a l1) (cons a l2).
+  | list_rel_cons a b l1 l2 : R a b ->list_rel R l1 l2 -> list_rel R (cons a l1) (cons b l2).
 
 Theorem transitive_list_rel A (R : Rel A A) : Transitive R -> Transitive (list_rel R).
 Proof.
@@ -79,9 +80,12 @@ Fixpoint ctx_equiv (Γ : ctx) : Rel (denote_ctx Γ) (denote_ctx Γ) :=
   | cons t Γ => prod_rel (types_equiv t) (ctx_equiv Γ)
   end.
 
+Definition comp_equiv_rutt {t MR} t1 t2 :=
+  rutt (mfix_pre_equiv MR) (mfix_post_equiv MR) (types_equiv t) t1 t2.
+
 Definition comp_equiv {t Γ MR} :=
     fun c1 c2 => forall hyps1 hyps2, ctx_equiv Γ hyps1 hyps2 ->
-              rutt (mfix_pre_equiv MR) (mfix_post_equiv MR) (types_equiv t) (c1 hyps1) (c2 hyps2).
+              comp_equiv_rutt (t := t) (MR := MR) (c1 hyps1) (c2 hyps2).
 
 Definition mfix_bodies_equiv {Γ MR R} :=
   fun bodies1 bodies2 => forall hyps1 hyps2 arg1 arg2, 
@@ -195,11 +199,11 @@ Lemma comp_equiv_call (t1 t2 : type) Γ MR R (xR : var R MR) (x : var (t1,t2) R)
   comp_equiv (MR := MR) (denote_value v1) (denote_value v2) ->
   comp_equiv (denote_comp (comp_call xR x v1)) (denote_comp (comp_call xR x v2)).
 Proof.
-  intros. red. intros.
+  intros. red. unfold comp_equiv_rutt. intros.
   simp denote_comp.
   eapply rutt_bind; eauto.
-  intros.
-  unfold call_term.
+  intros. eapply H; auto.
+  unfold call_term. intros.
   destruct (call_mrec x xR r1) as [c1 f1] eqn : Heq1.
   destruct (call_mrec x xR r2) as [c2 f2] eqn : Heq2. 
   setoid_rewrite bind_trigger. apply rutt_Vis.
@@ -209,14 +213,14 @@ Qed.
 
 
 Lemma pre_equiv_sum_rel MR R : 
-  forall c1 c2, mfix_pre_equiv (R :: MR) c1 c2 <-> sum_rel (call_frame_pre_equiv R) (mfix_pre_equiv MR) c1 c2.
+  eq_rel (mfix_pre_equiv (R :: MR)) (sum_rel (call_frame_pre_equiv R) (mfix_pre_equiv MR)).
 Proof.
   rewrite mfix_pre_equiv_equation_2.
   intros. reflexivity.
 Qed.
 
 Lemma post_equiv_sum_post_rel MR R : 
-  forall c1 c2 v1 v2, mfix_post_equiv (R :: MR) c1 c2 v1 v2 <-> SumPostRel (call_frame_post_equiv R) (mfix_post_equiv MR) c1 c2 v1 v2.
+  PostRelEq  (mfix_post_equiv (R :: MR)) (SumPostRel (call_frame_post_equiv R) (mfix_post_equiv MR)).
 Proof.
   rewrite mfix_post_equiv_equation_2.
   intros. reflexivity.
@@ -282,12 +286,394 @@ Proof.
   destruct types_equiv_trans_prod. auto.
 Qed.
 
+#[global] Instance comp_equiv_rutt_trans : forall t MR, Transitive (@comp_equiv_rutt t MR).
+Proof.
+  intros t MR. red. intros t1 t2 t3 Ht12 Ht23.
+  destruct types_equiv_trans_prod as [? [? ?]].
+  specialize (H0 MR) as [? ?].
+  eapply rutt_trans'; eauto.
+Qed.
+#[global] Instance comp_equiv_rutt_sym : forall t MR, Symmetric (@comp_equiv_rutt t MR).
+Proof.
+  intros t MR. red. intros t1 t2 Ht12.
+  destruct (types_equiv_sym_prod) as [? [? ?]].
+  specialize (H0 MR) as [? ?].
+  apply rutt_sym; auto.
+Qed.
+
+Lemma types_equiv_index_ctx:
+  forall (t : vtype) (Γ : ctx) (x : var t Γ) (hyps1 hyps2 : denote_ctx Γ),
+    ctx_equiv Γ hyps1 hyps2 -> types_equiv t (index_ctx x hyps1) (index_ctx x hyps2).
+Proof.
+  intros t Γ x. dependent induction x.
+  - intros. destruct hyps1; destruct hyps2. simp index_ctx.
+    red in H. destruct H. auto.
+  - intros. destruct hyps1; destruct hyps2. simp index_ctx. apply IHx.
+    red in H. destruct H. auto.
+Qed.
+Arguments lift_handler (MR1) {MR2}.
+
+Lemma mfix_pre_equiv_lift_handler:
+  forall (MR1 MR2 : mfix_ctx) (e1 e2 : denote_mrec_ctx (denote_mfix_ctx MR2)),
+    mfix_pre_equiv MR2 e1 e2 -> map_rel (lift_handler _) (lift_handler _) (mfix_pre_equiv (MR1 ++ MR2)) e1 e2.
+Proof.
+  intros MR1 MR2. unfold map_rel. revert MR2. induction MR1.
+  - intros. auto.
+  - setoid_rewrite lift_handler_equation_2. intros MR2 e1 e2 He12.
+    apply IHMR1 in He12. destruct (lift_handler MR1 e1). destruct (lift_handler MR1 e2).
+    constructor. auto.
+Qed.
+
+Lemma mfix_post_equiv_lift_handler:
+  forall (MR1 MR2 : mfix_ctx) (e1 e2 : denote_mrec_ctx (denote_mfix_ctx MR2)) 
+    (a : encodes e1) (b : encodes e2),
+    map_post_rel (lift_handler MR1) (lift_handler MR1) (mfix_post_equiv (MR1 ++ MR2)) e1 e2 a b ->
+    mfix_post_equiv MR2 e1 e2 a b.
+Proof.
+  intros MR1 MR2. unfold map_post_rel. revert MR2. induction MR1.
+  - repeat setoid_rewrite lift_handler_equation_1. intros.
+    decompose record H. subst. auto.
+  - repeat setoid_rewrite lift_handler_equation_2. intros.
+    specialize (IHMR1 MR2 e1 e2 a0 b). simp lift_handler in H.
+    destruct (lift_handler MR1 e1). destruct (lift_handler MR1 e2).
+    apply IHMR1. decompose record H. subst. eexists. eexists.
+    repeat split; eauto.
+    simpl app in H3. rewrite mfix_post_equiv_equation_2 in H3.
+    dependent destruction H3. auto.
+Qed.
+
+Lemma perm_nil_cons1:
+  forall A (l : list A), perm [] l -> l = [].
+Proof.
+  intros A l Hperm. dependent induction Hperm; eauto.
+Qed.
+
+Lemma perm_nil_cons2:
+  forall A (l : list A), perm l [] -> l = [].
+Proof.
+  intros A l Hperm. dependent induction Hperm; eauto.
+Qed.
+
+Lemma perm_nil_cons1': 
+  forall A (a : A) (t : list A), perm [] (a :: t) -> False.
+Proof.
+  intros. apply perm_nil_cons1 in X. discriminate.
+Qed.
+
+Lemma perm_nil_cons2' :
+  forall A (a : A) (t : list A), perm (a :: t) [] -> False.
+Proof.
+  intros. apply perm_nil_cons2 in X. discriminate.
+Qed.
+
+Lemma unfold_denote_mfix_ctx R MR : 
+  denote_mfix_ctx (R :: MR) = (denote_call_frame R && encodes_call_frame R) :: denote_mfix_ctx MR.
+Proof. reflexivity. Qed.
+Transparent perm_map.
+Lemma mfix_pre_equiv_perm_handler:
+  forall (MR1 MR2 : mfix_ctx) (Hperm : perm MR1 MR2) (e1 e2 : denote_mrec_ctx (denote_mfix_ctx MR1)),
+    mfix_pre_equiv MR1 e1 e2 ->
+    map_rel (perm_handler (denote_mfix_ctx MR1) (denote_mfix_ctx MR2) (perm_denote Hperm))
+            (perm_handler (denote_mfix_ctx MR1) (denote_mfix_ctx MR2) (perm_denote Hperm))
+            (mfix_pre_equiv MR2) e1 e2.
+Proof.
+  intros MR1 MR2 Hperm. unfold map_rel. dependent induction Hperm.
+  - intros. contradiction.
+  - intros. rewrite mfix_pre_equiv_equation_2 in H. dependent destruction H.
+    + simp perm_handler. unfold perm_denote. repeat simp perm_map.
+      simpl perm_map. simp perm_handler.
+      setoid_rewrite perm_handler_equation_5. constructor; auto.
+    + unfold perm_denote. simpl perm_map.
+      apply IHHperm in H. rewrite mfix_pre_equiv_equation_2. simpl List.map.
+      destruct (perm_handler (denote_mfix_ctx l1) (denote_mfix_ctx l2) (perm_denote Hperm) b1)
+        eqn : Heq1;
+      destruct (perm_handler (denote_mfix_ctx l1) (denote_mfix_ctx l2) (perm_denote Hperm) b2)
+        eqn : Heq2. cbn in H.
+      setoid_rewrite perm_handler_equation_6; setoid_rewrite Heq1; setoid_rewrite Heq2.
+      constructor; auto.
+ - repeat rewrite mfix_pre_equiv_equation_2. intros e1 e2 He12.
+   dependent destruction He12. 2 : dependent destruction H.
+   + unfold perm_denote. simpl perm_map. 
+     setoid_rewrite perm_handler_equation_7. repeat constructor. auto.
+   + unfold perm_denote. simpl perm_map. setoid_rewrite perm_handler_equation_8.
+     constructor. auto.
+   + unfold perm_denote. simpl perm_map. 
+     apply IHHperm in H.
+     destruct (perm_handler (denote_mfix_ctx l1) (denote_mfix_ctx l2) (perm_denote Hperm) b1)
+              eqn : Heq1;
+     destruct (perm_handler (denote_mfix_ctx l1) (denote_mfix_ctx l2) (perm_denote Hperm) b2)
+              eqn : Heq2. cbn in H.
+     setoid_rewrite perm_handler_equation_9; setoid_rewrite Heq1; setoid_rewrite Heq2.
+     repeat constructor. auto.
+ - intros e1 e2 He12. unfold perm_denote. simpl perm_map.
+   apply IHHperm1 in He12.
+   destruct (perm_handler (denote_mfix_ctx l1) (denote_mfix_ctx l2) (perm_denote Hperm1) e1)
+     eqn : Heq1;
+   destruct (perm_handler (denote_mfix_ctx l1) (denote_mfix_ctx l2) (perm_denote Hperm1) e2)
+     eqn : Heq2. cbn in He12.
+   (* might be worth rethinking the whole mapE handler thing 
+      of using equations to do weird safe typecasts,
+
+      or perhaps think carefully about how this might be refactored into two more normal lemmas
+    *)
+   destruct l1; destruct l3.
+   + cbv in e1. contradiction. 
+   + exfalso. clear - Hperm1 Hperm2. eapply perm_nil_cons1'.
+     eapply perm_trans; eauto.
+   + exfalso. clear - Hperm1 Hperm2. eapply perm_nil_cons2'.
+     eapply perm_trans; eauto.
+   + specialize (IHHperm2 x x0 He12). specialize (IHHperm1 e1 e2).
+     setoid_rewrite perm_handler_equation_10; setoid_rewrite Heq1; setoid_rewrite Heq2.
+     destruct (perm_handler (denote_mfix_ctx l2) (denote_mfix_ctx (l0 :: l3))
+                     (perm_denote Hperm2) x) eqn : Heq3.
+     destruct ((perm_handler (denote_mfix_ctx l2) (denote_mfix_ctx (l0 :: l3))
+                     (perm_denote Hperm2) x0)) eqn : Heq4.
+     setoid_rewrite Heq3. setoid_rewrite Heq4.
+     simpl projT1. auto.
+Qed.
+#[local] Instance eq_sub_eq {A} : subrelation (@eq A) eq.
+Proof.
+  repeat intro. auto.
+Qed.
 (*
-Lemma types_equiv_comp_refl_prop : 
+#[local] Instance eq_sub_impl {A : Prop} : subrelation (@eq A) (@impl A).
+*)
+Lemma mfix_post_equiv_perm_handler:
+  forall (MR1 MR2 : mfix_ctx) (Hperm : perm MR1 MR2) (e1 e2 : denote_mrec_ctx (denote_mfix_ctx MR1))
+    (a : encodes e1) (b : encodes e2),
+    map_post_rel (perm_handler (denote_mfix_ctx MR1) (denote_mfix_ctx MR2) (perm_denote Hperm))
+                 (perm_handler (denote_mfix_ctx MR1) (denote_mfix_ctx MR2) (perm_denote Hperm))
+                 (mfix_post_equiv MR2) e1 e2 a b -> mfix_post_equiv MR1 e1 e2 a b.
+Proof.
+  intros MR1 MR2 Hperm. unfold map_post_rel. dependent induction Hperm.
+  - intros. contradiction.
+  - unfold perm_denote. simpl perm_map.
+    intros. simp perm_handler in H.
+    destruct e1; destruct e2.
+    + cbn in H. repeat rewrite perm_handler_equation_5 in H.
+      destruct H as [a' [b' [Ha' [Hb' H] ] ] ].
+      subst. dependent destruction H. constructor; eauto.
+    + match goal with
+      | H : let 'd' && f1 := ?x in _ |- _ => destruct x eqn : Heq1 end.
+      match goal with
+      | H : let 'd' && f1 := ?x in _ |- _ => destruct x eqn : Heq2 end.
+      setoid_rewrite perm_handler_equation_5 in Heq1.
+      setoid_rewrite perm_handler_equation_6 in Heq2.
+      match goal with
+      | H : (let 'd' && f1 := ?x in _) = _ |- _ => destruct x end.
+      injection Heq1. injection Heq2. intros. subst.
+      decompose record H. rewrite mfix_post_equiv_equation_2 in H4. dependent destruction H4.
+    + match goal with
+      | H : let 'd' && f1 := ?x in _ |- _ => destruct x eqn : Heq1 end.
+      match goal with
+      | H : let 'd' && f1 := ?x in _ |- _ => destruct x eqn : Heq2 end.
+      setoid_rewrite perm_handler_equation_5 in Heq2.
+      setoid_rewrite perm_handler_equation_6 in Heq1.
+      match goal with
+      | H : (let 'd' && f1 := ?x in _) = _ |- _ => destruct x end.
+      injection Heq1. injection Heq2. intros. subst.
+      decompose record H. rewrite mfix_post_equiv_equation_2 in H4. dependent destruction H4.
+    + match goal with
+      | H : let 'd' && f1 := ?x in _ |- _ => destruct x eqn : Heq1 end.
+      match goal with
+      | H : let 'd' && f1 := ?x in _ |- _ => destruct x eqn : Heq2 end.
+      setoid_rewrite perm_handler_equation_6 in Heq1.
+      setoid_rewrite perm_handler_equation_6 in Heq2.
+      match goal with
+      | H : (let 'd' && f1 := ?x in _) = _ |- _ => destruct x eqn : Heq3 end.
+      match goal with
+      | H : (let 'd' && f1 := ?x in _) = _ |- _ => destruct x eqn : Heq4 end.
+      destruct H as [a' [b' [Ha' [Hb' H] ] ]].
+      subst. rewrite mfix_post_equiv_equation_2.
+      constructor. 
+      specialize (IHHperm d d0 (e a') (e0 b')).
+      setoid_rewrite Heq4 in IHHperm. setoid_rewrite Heq3 in IHHperm.
+      apply IHHperm. injection Heq2. intros. subst. injection Heq1.
+      intros. subst. inj_existT. subst.
+      exists a'. exists b'. do 2 split; auto. rewrite mfix_post_equiv_equation_2 in H. 
+      dependent destruction H. auto.
+  - (* the rest, unfortunately will likely be similarly painful come back to this
+       on monday *)
+    intros e1 e2 a b He12.
+    match goal with
+      | H : let 'd' && f1 := ?x in _ |- _ => destruct x eqn : Heq1 end.
+    match goal with
+      | H : let 'd' && f1 := ?x in _ |- _ => destruct x eqn : Heq2 end.
+    destruct He12 as [a' [b' [Ha' [Hb' H]] ]]. subst.
+    unfold perm_denote in Heq1, Heq2. simpl perm_map in Heq1, Heq2.
+    repeat rewrite mfix_post_equiv_equation_2 in H.
+    repeat destruct e1 as [e1 | e1].
+    + setoid_rewrite perm_handler_equation_7 in Heq1. injection Heq1. intros. subst.
+      inj_existT. subst.
+      repeat dependent destruction H.
+      repeat destruct e2 as [e2 | e2].
+      * setoid_rewrite perm_handler_equation_7 in Heq2. injection Heq2.
+        intros. subst. inj_existT. subst. constructor; auto.
+      * setoid_rewrite perm_handler_equation_8 in Heq2. discriminate.
+      * setoid_rewrite perm_handler_equation_9 in Heq2. 
+        match goal with
+        | H : (let 'd' && f1 := ?x in _) = _ |- _ => destruct x; discriminate end.
+    + setoid_rewrite perm_handler_equation_8 in Heq1. injection Heq1.
+      intros. subst. inj_existT. subst.
+      dependent destruction H.
+      repeat destruct e2 as [e2 | e2].
+      * setoid_rewrite perm_handler_equation_7 in Heq2; discriminate.
+      * setoid_rewrite perm_handler_equation_8 in Heq2. injection Heq2.
+        intros. subst. inj_existT. subst.
+        repeat constructor; auto.
+      * setoid_rewrite perm_handler_equation_9 in Heq2.
+         match goal with
+        | H : (let 'd' && f1 := ?x in _) = _ |- _ => destruct x; discriminate end.
+    + setoid_rewrite perm_handler_equation_9 in Heq1.
+      match goal with
+      | H : (let 'd' && f1 := ?x in _) = _ |- _ => destruct x eqn : Heq3 end.
+      injection Heq1. intros. subst. inj_existT. subst.
+      repeat dependent destruction H.
+      repeat destruct e2 as [e2 | e2].
+      * clear Heq3. setoid_rewrite perm_handler_equation_7 in Heq2.
+        discriminate.
+      * clear Heq3. setoid_rewrite perm_handler_equation_8 in Heq2.
+        discriminate.
+      * setoid_rewrite perm_handler_equation_9 in Heq2.
+        match goal with
+        | H : (let 'd' && f1 := ?x in _) = _ |- _ => destruct x eqn : Heq4 end.
+        specialize (IHHperm e1 e2 (e a') (e0 b')).
+        setoid_rewrite Heq3 in IHHperm. setoid_rewrite Heq4 in IHHperm.
+        repeat rewrite mfix_post_equiv_equation_2.
+        repeat constructor. apply IHHperm.
+        injection Heq2. intros. subst. inj_existT. subst.
+        exists a'. exists b'. repeat split; auto.
+  - intros e1 e2 a b. unfold perm_denote. simpl perm_map. intros IHe12.
+    apply IHHperm1. clear IHHperm1.
+    match goal with
+      | |- let 'd' && f1 := ?x in _ => destruct x eqn : Heq1 end.
+      match goal with
+      | |- let 'd' && f1 := ?x in _ => destruct x eqn : Heq2 end.
+    match goal with
+      | H : (let 'd' && f1 := ?x in _) |- _ => destruct x eqn : Heq3 end.
+    match goal with
+      | H : (let 'd' && f1 := ?x in _) |- _ => destruct x eqn : Heq4 end.
+    destruct l1; destruct l3; try contradiction.
+    setoid_rewrite perm_handler_equation_10 in Heq3.
+    setoid_rewrite perm_handler_equation_10 in Heq4.
+    destruct IHe12 as [a' [b' [Ha' [Hb' H] ] ] ].
+    subst. rewrite mfix_post_equiv_equation_2 in H.
+    setoid_rewrite Heq1 in Heq3. setoid_rewrite Heq2 in Heq4.
+    dependent destruction H.
+    * match goal with
+      | H : (let 'd' && f1 := ?x in _) = _ |- _ => destruct x eqn : Heq5 end.
+      match goal with
+      | H : (let 'd' && f1 := ?x in _) = _ |- _ => destruct x eqn : Heq6 end.
+      injection Heq4. intros. subst. inj_existT. subst.
+      injection Heq3. intros. subst. inj_existT. subst.
+      exists (e8 a). exists (e7 b). repeat split; auto.
+      eapply IHHperm2. clear H0 H1.
+      match goal with
+      | |- let 'd' && f1 := ?x in _ => destruct x eqn : Heq7 end.
+      match goal with
+      | |- let 'd' && f1 := ?x in _ => destruct x eqn : Heq8 end.
+      setoid_rewrite Heq8 in Heq5. setoid_rewrite Heq7 in Heq6.
+      injection Heq5. injection Heq6. intros. subst. inj_existT.
+      subst. exists a. exists b. repeat split; auto. constructor; auto.
+    * match goal with
+      | H : (let 'd' && f1 := ?x in _) = _ |- _ => destruct x eqn : Heq5 end.
+      match goal with
+      | H : (let 'd' && f1 := ?x in _) = _ |- _ => destruct x eqn : Heq6 end.
+      injection Heq4. intros. subst. inj_existT. subst.
+      injection Heq3. intros. subst. inj_existT. subst.
+      clear H0 H1. exists (e6 a). exists (e5 b). repeat split; auto.
+      eapply IHHperm2.
+      match goal with
+      | |- let 'd' && f1 := ?x in _ => destruct x eqn : Heq7 end.
+      match goal with
+      | |- let 'd' && f1 := ?x in _ => destruct x eqn : Heq8 end.
+      setoid_rewrite Heq8 in Heq5. setoid_rewrite Heq7 in Heq6.
+      injection Heq6. injection Heq5. intros. subst. inj_existT. subst.
+      exists a. exists b. repeat split; auto. constructor; auto.
+Qed.
+
+Lemma types_equiv_comp_refl_prod : 
   (forall t Γ MR (c : comp t Γ MR), comp_equiv (denote_comp c) (denote_comp c)) /\
   (forall t Γ (v : value t Γ), forall MR, comp_equiv (MR := MR) (denote_value v) (denote_value v)) /\
-    (* maybe I should look carefully at mfix_bodies type signature, maybe I can change it and get better results*)
-    (forall Γ MR' R (bodies : mfix_bodies Γ MR' R) MR, MR' = R :: MR -> mfix_bodies_equiv (denote_bodies bodies) (denote_bodies bodies)).
+    (forall Γ MR R R' (bodies : mfix_bodies Γ MR R R'), mfix_bodies_equiv (denote_bodies bodies) (denote_bodies bodies)).
 Proof.
+  unfold comp_equiv, comp_equiv_rutt.
   apply comp_value_mutind.
-*)
+  - repeat intro. do 2 rewrite denote_value_equation_1. apply rutt_Ret. simp types_equiv. auto.
+  - repeat intro. do 2 rewrite denote_value_equation_2. apply rutt_Ret. simp types_equiv. constructor.
+  - intros t Γ vh Hhv vt Hvt MR. specialize (Hhv MR). specialize (Hvt MR).
+    intros hyps1 hyps2 Hhyps. setoid_rewrite denote_value_equation_3.
+    eapply rutt_bind; eauto; intros. eapply rutt_bind; eauto. intros. apply rutt_Ret.
+    simp types_equiv. constructor; auto.
+  - intros t1 t2 Γ v1 Hv1 v2 Hv2 MR hyps1 hyps2 Hhyps. setoid_rewrite denote_value_equation_4.
+    eapply rutt_bind; try eapply Hv1; eauto. intros. eapply rutt_bind; try eapply Hv2; eauto.
+    intros. apply rutt_Ret. constructor; auto.
+  - intros t1 t2 Γ MR cbody Hcbody MR' hyps1 hyps2 Hhyps. setoid_rewrite denote_value_equation_5.
+    apply rutt_Ret. simp types_equiv. intros. apply Hcbody. split; auto.
+  - intros t Γ x MR hyps1 hyps2 Hhyps. setoid_rewrite denote_value_equation_6.
+    apply rutt_Ret. apply types_equiv_index_ctx; auto.
+  - repeat intro. simp denote_comp.
+  - intros t1 t2 Γ MR c1 Hc1 c2 Hc2 hyps1 hyps2 Hhyps.
+    simp denote_comp. eapply rutt_bind; eauto. intros. eapply Hc2. split; auto.
+  - intros ? ? ? ? Hvn ? HcZ ? HcS ? ? ?. simp denote_comp.
+    eapply rutt_bind; try eapply Hvn; eauto. intros n1 n2 Hn12. simp types_equiv in Hn12. subst.
+    destruct n2; eauto. eapply HcS. split; auto. reflexivity.
+  - intros ? ? ? ? ? Hvl ? Hcnil ? Hccons ? ? ?. simp denote_comp.
+    eapply rutt_bind; try eapply Hvl; eauto. intros l1 l2 Hl12. simp types_equiv in Hl12.
+    dependent destruction Hl12; eauto. eapply Hccons. do 2 (split; auto).
+  - intros ? ? ? ? ? ? Hvp ? Hes ? ? ?. simp denote_comp.
+    eapply rutt_bind; try apply Hvp; auto. intros. simp types_equiv in H0.
+    dependent destruction H0. destruct r1. destruct r2. cbn in *.
+    apply Hes. repeat (split; auto).
+  - intros ? ? ? ? ? Hvf ? Hvarg ? ? ?. simp denote_comp.
+    eapply rutt_bind; try apply Hvf; auto. intros f g Hfg.
+    eapply rutt_bind. apply Hvarg; auto. exact Hfg.
+  - intros. apply comp_equiv_call. repeat intro. eapply H. auto. auto.
+  - intros t Γ MR R bodies Hbodies c Hc hyps1 hyps2 Hhyps.
+    simp denote_comp. 
+    eapply interp_mrec_rutt with (RPreInv := call_frame_pre_equiv R) (RPostInv := call_frame_post_equiv R). 
+    intros. eapply Hbodies; eauto.
+    apply Hc. auto.
+  - intros t Γ MR1 MR2 c Hc hyps1 hyps2 Hhyps. simp denote_comp. apply mapE_rutt.
+    eapply rutt_mon; try eapply Hc; eauto. apply mfix_pre_equiv_lift_handler.
+    apply mfix_post_equiv_lift_handler.
+  - intros t Γ MR1 MR2 Hperm c Hc hyps1 hyps2 Hhyps. simp denote_comp. apply mapE_rutt.
+    eapply rutt_mon; try apply Hc; eauto.
+    apply mfix_pre_equiv_perm_handler.
+    apply mfix_post_equiv_perm_handler.  
+  - repeat intro. simp denote_bodies. inversion arg1.
+  - intros Γ MR t1 t2 R R' body Hbody bodies Hbodies hyps1 hyps2 args1 args2 Hhyps Hargs.
+    rewrite call_frame_pre_equiv_equation_2 in Hargs. dependent destruction Hargs.
+    + setoid_rewrite denote_bodies_equation_2. red in Hbody.
+      eapply rutt_mon; try eapply Hbody; eauto.
+      * intros. constructor. auto.
+      * split; auto.
+    + setoid_rewrite denote_bodies_equation_3. eapply rutt_mon; try eapply Hbodies; eauto.
+      intros. constructor. auto.
+Qed.
+
+Theorem types_equiv_comp_refl : forall t Γ MR (c : comp t Γ MR), comp_equiv (denote_comp c) (denote_comp c).
+Proof. destruct types_equiv_comp_refl_prod as [? [? ?]]; auto. Qed.
+
+Theorem types_equiv_value_refl : forall t Γ MR (v : value t Γ), comp_equiv (MR := MR) (denote_value v) (denote_value v).
+Proof. destruct types_equiv_comp_refl_prod as [? [? ?]]; intros; auto. Qed.
+
+Theorem types_equiv_mfix_bodies_refl : forall Γ MR R R' (bodies : mfix_bodies Γ MR R R'), mfix_bodies_equiv (denote_bodies bodies) (denote_bodies bodies).
+Proof. destruct types_equiv_comp_refl_prod as [? [? ?]]; intros; auto. Qed.
+
+#[global] Instance ctx_equiv_sym Γ : Symmetric (ctx_equiv Γ).
+Proof.
+  red. induction Γ.
+  - intros. auto.
+  - intros. simpl ctx_equiv in *. dependent destruction H.
+    constructor; auto. symmetry. auto.
+Qed.
+
+#[global] Instance ctx_equiv_trans Γ : Transitive (ctx_equiv Γ).
+Proof.
+  red. induction Γ.
+  - intros. auto.
+  - intros. simpl ctx_equiv in *. dependent destruction H.
+    dependent destruction H0. constructor; eauto.
+    etransitivity; eauto.
+Qed.
